Working on interpreter

cfrontend/Cexec.v
@@ -18,6 +18,8 @@ Require Import String Coqlib Decidableplus.
 Require Import Errors Maps Integers Floats.
 Require Import AST Values Memory Events Globalenvs Builtins Determinism.
 Require Import Ctypes Cop Csyntax Csem.
+Require Import Tags.
+Require Import List. Import ListNotations.
 Require Cstrategy.
 
 Local Open Scope string_scope.
@@ -53,7 +55,22 @@ Notation " 'check' A ; B" := (if A then B else nil)
   (at level 200, A at level 100, B at level 200)
   : list_monad_scope.
 
-Definition is_val (a: expr) : option (val * type) :=
+Module Cexec (T:Tag) (P:Policy T).
+  Module TLib := TagLib T.
+  Import TLib.
+  Module Csem := Csem T P.
+  Import Csem.
+  Import Csyntax.
+  Import Cop.
+  Import Deterministic.
+  Import Behaviors.
+  Import Smallstep.
+  Import Events.
+  Import Genv.
+  Import Mem.
+  Import P.
+  
+Definition is_val (a: expr) : option (atom * type) :=
   match a with
   | Eval v ty => Some(v, ty)
   | _ => None
@@ -65,21 +82,21 @@ Proof.
   intros until ty. destruct a; simpl; congruence.
 Qed.
 
-Definition is_loc (a: expr) : option (block * ptrofs * bitfield * type) :=
+Definition is_loc (a: expr) : option (block * ptrofs * tag * bitfield * type) :=
   match a with
-  | Eloc b ofs bf ty => Some(b, ofs, bf, ty)
+  | Eloc b ofs pt bf ty => Some(b, ofs, pt, bf, ty)
   | _ => None
   end.
 
 Lemma is_loc_inv:
-  forall a b ofs bf ty, is_loc a = Some(b, ofs, bf, ty) -> a = Eloc b ofs bf ty.
+  forall a b ofs pt bf ty, is_loc a = Some(b, ofs, pt, bf, ty) -> a = Eloc b ofs pt bf ty.
 Proof.
   intros until ty. destruct a; simpl; congruence.
 Qed.
 
 Local Open Scope option_monad_scope.
 
-Fixpoint is_val_list (al: exprlist) : option (list (val * type)) :=
+Fixpoint is_val_list (al: exprlist) : option (list (atom * type)) :=
   match al with
   | Enil => Some nil
   | Econs a1 al => do vt1 <- is_val a1; do vtl <- is_val_list al; Some(vt1::vtl)
@@ -94,23 +111,24 @@ Defined.
 
 Section EXEC.
 
-Variable ge: genv.
+Variable ge: gcenv.
 
-Definition eventval_of_val (v: val) (t: typ) : option eventval :=
+Definition eventval_of_val (a: atom) (t: typ) : option eventval :=
+  let '(v,vt) := a in
   match v with
-  | Vint i => check (typ_eq t AST.Tint); Some (EVint i)
-  | Vfloat f => check (typ_eq t AST.Tfloat); Some (EVfloat f)
-  | Vsingle f => check (typ_eq t AST.Tsingle); Some (EVsingle f)
-  | Vlong n => check (typ_eq t AST.Tlong); Some (EVlong n)
+  | Vint i => check (typ_eq t AST.Tint); Some (EVint i vt)
+  | Vfloat f => check (typ_eq t AST.Tfloat); Some (EVfloat f vt)
+  | Vsingle f => check (typ_eq t AST.Tsingle); Some (EVsingle f vt)
+  | Vlong n => check (typ_eq t AST.Tlong); Some (EVlong n vt)
   | Vptr b ofs =>
-      do id <- Genv.invert_symbol ge b;
-      check (Genv.public_symbol ge id);
+      do id <- Genv.invert_symbol (fst ge) b;
+      check (Genv.public_symbol (fst ge) id);
       check (typ_eq t AST.Tptr);
-      Some (EVptr_global id ofs)
+      Some (EVptr_global id ofs vt)
   | _ => None
   end.
 
-Fixpoint list_eventval_of_val (vl: list val) (tl: list typ) : option (list eventval) :=
+Fixpoint list_eventval_of_val (vl: list atom) (tl: list typ) : option (list eventval) :=
   match vl, tl with
   | nil, nil => Some nil
   | v1::vl, t1::tl =>
@@ -120,17 +138,18 @@ Fixpoint list_eventval_of_val (vl: list val) (tl: list typ) : option (list event
   | _, _ => None
   end.
 
-Definition val_of_eventval (ev: eventval) (t: typ) : option val :=
+Definition val_of_eventval (ev: eventval) (t: typ) : option atom :=
   match ev with
-  | EVint i => check (typ_eq t AST.Tint); Some (Vint i)
-  | EVfloat f => check (typ_eq t AST.Tfloat); Some (Vfloat f)
-  | EVsingle f => check (typ_eq t AST.Tsingle); Some (Vsingle f)
-  | EVlong n => check (typ_eq t AST.Tlong); Some (Vlong n)
-  | EVptr_global id ofs =>
-      check (Genv.public_symbol ge id);
+  | EVint i vt => check (typ_eq t AST.Tint); Some (Vint i, vt)
+  | EVfloat f vt => check (typ_eq t AST.Tfloat); Some (Vfloat f, vt)
+  | EVsingle f vt => check (typ_eq t AST.Tsingle); Some (Vsingle f, vt)
+  | EVlong n vt => check (typ_eq t AST.Tlong); Some (Vlong n, vt)
+  | EVptr_global id ofs vt =>
+      check (Genv.public_symbol (fst ge) id);
       check (typ_eq t AST.Tptr);
-      do b <- Genv.find_symbol ge id;
-      Some (Vptr b ofs)
+      do bt <- Genv.find_symbol (fst ge) id;
+      let '(b,pt) := bt in
+      Some (Vptr b ofs, pt)
   end.
 
 Ltac mydestr :=
@@ -140,18 +159,20 @@ Ltac mydestr :=
   | [ |- match ?x with Some _ => _ | None => _ end = Some _ -> _ ] => destruct x eqn:?; mydestr
   | [ |- match ?x with true => _ | false => _ end = Some _ -> _ ] => destruct x eqn:?; mydestr
   | [ |- match ?x with left _ => _ | right _ => _ end = Some _ -> _ ] => destruct x; mydestr
+  | [ |- (let (_, _) := ?x in _) = Some _ -> _ ] => destruct x; mydestr
   | _ => idtac
   end.
 
 Lemma eventval_of_val_sound:
-  forall v t ev, eventval_of_val v t = Some ev -> eventval_match ge ev t v.
-Proof.
+  forall v t ev, eventval_of_val v t = Some ev -> eventval_match (fst ge) ev t v.
+Admitted.
+(*Proof.
   intros until ev. destruct v; simpl; mydestr; constructor.
   auto. apply Genv.invert_find_symbol; auto.
-Qed.
+Qed.*)
 
 Lemma eventval_of_val_complete:
-  forall ev t v, eventval_match ge ev t v -> eventval_of_val v t = Some ev.
+  forall ev t v, eventval_match (fst ge) ev t v -> eventval_of_val v t = Some ev.
 Proof.
   induction 1; simpl.
 - auto.
@@ -163,30 +184,31 @@ Proof.
 Qed.
 
 Lemma list_eventval_of_val_sound:
-  forall vl tl evl, list_eventval_of_val vl tl = Some evl -> eventval_list_match ge evl tl vl.
+  forall vl tl evl, list_eventval_of_val vl tl = Some evl -> eventval_list_match (fst ge) evl tl vl.
 Proof with try discriminate.
   induction vl; destruct tl; simpl; intros; inv H.
   constructor.
-  destruct (eventval_of_val a t) as [ev1|] eqn:?...
+  destruct (eventval_of_val a t0) as [ev1|] eqn:?...
   destruct (list_eventval_of_val vl tl) as [evl'|] eqn:?...
   inv H1. constructor. apply eventval_of_val_sound; auto. eauto.
 Qed.
 
 Lemma list_eventval_of_val_complete:
-  forall evl tl vl, eventval_list_match ge evl tl vl -> list_eventval_of_val vl tl = Some evl.
+  forall evl tl vl, eventval_list_match (fst ge) evl tl vl -> list_eventval_of_val vl tl = Some evl.
 Proof.
   induction 1; simpl. auto.
   rewrite (eventval_of_val_complete _ _ _ H). rewrite IHeventval_list_match. auto.
 Qed.
 
 Lemma val_of_eventval_sound:
-  forall ev t v, val_of_eventval ev t = Some v -> eventval_match ge ev t v.
-Proof.
+  forall ev t v, val_of_eventval ev t = Some v -> eventval_match (fst ge) ev t v.
+Admitted.
+(*Proof.
   intros until v. destruct ev; simpl; mydestr; constructor; auto.
-Qed.
+Qed.*)
 
 Lemma val_of_eventval_complete:
-  forall ev t v, eventval_match ge ev t v -> val_of_eventval ev t = Some v.
+  forall ev t v, eventval_match (fst ge) ev t v -> val_of_eventval ev t = Some v.
 Proof.
   induction 1; simpl.
 - auto.
@@ -197,93 +219,100 @@ Proof.
 Qed.
 
 (** Volatile memory accesses. *)
-
 Definition do_volatile_load (w: world) (chunk: memory_chunk) (m: mem) (b: block) (ofs: ptrofs)
-                             : option (world * trace * val) :=
-  if Genv.block_is_volatile ge b then
-    do id <- Genv.invert_symbol ge b;
+                             : option (world * trace * atom * (list tag)) :=
+  if (b =? dummy)%positive && Genv.addr_is_volatile (fst ge) ofs then
+    do id <- Genv.invert_symbol (fst ge) b;
     match nextworld_vload w chunk id ofs with
     | None => None
     | Some(res, w') =>
         do vres <- val_of_eventval res (type_of_chunk chunk);
-        Some(w', Event_vload chunk id ofs res :: nil, Val.load_result chunk vres)
+        Some(w', Event_vload chunk id ofs res :: nil,
+              atom_map (Val.load_result chunk) vres, load_ltags chunk m b ofs)
     end
   else
     do v <- Mem.load chunk m b (Ptrofs.unsigned ofs);
     Some(w, E0, v).
 
-Definition do_volatile_store (w: world) (chunk: memory_chunk) (m: mem) (b: block) (ofs: ptrofs) (v: val)
-                             : option (world * trace * mem * val) :=
-  if Genv.block_is_volatile ge b then
-    do id <- Genv.invert_symbol ge b;
-    do ev <- eventval_of_val (Val.load_result chunk v) (type_of_chunk chunk);
+Definition do_volatile_store (w: world) (chunk: memory_chunk) (m: mem) (b: block) (ofs: ptrofs) (v: atom) (lts: list tag)
+                             : option (world * trace * mem * atom) :=
+  if (b =? dummy)%positive && Genv.addr_is_volatile (fst ge) ofs then
+    do id <- Genv.invert_symbol (fst ge) b;
+    do ev <- eventval_of_val (atom_map (Val.load_result chunk) v) (type_of_chunk chunk);
     do w' <- nextworld_vstore w chunk id ofs ev;
     Some(w', Event_vstore chunk id ofs ev :: nil, m, v)
   else
-    do m' <- Mem.store chunk m b (Ptrofs.unsigned ofs) v;
+    do m' <- Mem.store chunk m b (Ptrofs.unsigned ofs) v lts;
     Some(w, E0, m', v).
 
 Lemma do_volatile_load_sound:
-  forall w chunk m b ofs w' t v,
+  forall w chunk m b ofs w' t v lts,
   do_volatile_load w chunk m b ofs = Some(w', t, v) ->
-  volatile_load ge chunk m b ofs t v /\ possible_trace w t w'.
-Proof.
+  volatile_load (fst ge) chunk m b ofs t v lts /\ possible_trace w t w'.
+Admitted.
+(*Proof.
   intros until v. unfold do_volatile_load. mydestr.
   destruct p as [ev w'']. mydestr.
   split. constructor; auto. apply Genv.invert_find_symbol; auto.
   apply val_of_eventval_sound; auto.
   econstructor. constructor; eauto. constructor.
   split. constructor; auto. constructor.
-Qed.
+Qed.*)
 
 Lemma do_volatile_load_complete:
-  forall w chunk m b ofs w' t v,
-  volatile_load ge chunk m b ofs t v -> possible_trace w t w' ->
+  forall w chunk m b ofs w' t v lts,
+  volatile_load (fst ge) chunk m b ofs t v lts -> possible_trace w t w' ->
   do_volatile_load w chunk m b ofs = Some(w', t, v).
 Proof.
   unfold do_volatile_load; intros. inv H; simpl in *.
   rewrite H1. rewrite (Genv.find_invert_symbol _ _ H2). inv H0. inv H8. inv H6. rewrite H9.
   rewrite (val_of_eventval_complete _ _ _ H3). auto.
   rewrite H1. rewrite H2. inv H0. auto.
+  destruct b eqn:E.
+  - simpl. rewrite H2. inv H0. auto.
+  - simpl. rewrite H2. inv H0. auto.
+  - unfold dummy in *. contradiction.
 Qed.
 
 Lemma do_volatile_store_sound:
-  forall w chunk m b ofs v w' t m' v',
-  do_volatile_store w chunk m b ofs v = Some(w', t, m', v') ->
-  volatile_store ge chunk m b ofs v t m' /\ possible_trace w t w' /\ v' = v.
-Proof.
+  forall w chunk m b ofs v w' t m' v' lts,
+  do_volatile_store w chunk m b ofs v lts = Some(w', t, m', v') ->
+  volatile_store (fst ge) chunk m b ofs v lts t m' /\ possible_trace w t w' /\ v' = v.
+Admitted.
+(*Proof.
   intros until v'. unfold do_volatile_store. mydestr.
   split. constructor; auto. apply Genv.invert_find_symbol; auto.
   apply eventval_of_val_sound; auto.
   split. econstructor. constructor; eauto. constructor. auto.
   split. constructor; auto. split. constructor. auto.
-Qed.
+Qed.*)
 
 Lemma do_volatile_store_complete:
-  forall w chunk m b ofs v w' t m',
-  volatile_store ge chunk m b ofs v t m' -> possible_trace w t w' ->
-  do_volatile_store w chunk m b ofs v = Some(w', t, m', v).
-Proof.
+  forall w chunk m b ofs v w' t m' lts,
+  volatile_store (fst ge) chunk m b ofs v lts t m' -> possible_trace w t w' ->
+  do_volatile_store w chunk m b ofs v lts = Some(w', t, m', v).
+Admitted.
+(*Proof.
   unfold do_volatile_store; intros. inv H; simpl in *.
   rewrite H1. rewrite (Genv.find_invert_symbol _ _ H2).
   rewrite (eventval_of_val_complete _ _ _ H3).
   inv H0. inv H8. inv H6. rewrite H9. auto.
   rewrite H1. rewrite H2. inv H0. auto.
-Qed.
+Qed.*)
 
 (** Accessing locations *)
 
-Definition do_deref_loc (w: world) (ty: type) (m: mem) (b: block) (ofs: ptrofs) (bf: bitfield) : option (world * trace * val) :=
+Definition do_deref_loc (w: world) (ty: type) (m: mem) (b: block) (ofs: ptrofs) (pt:tag) (bf: bitfield) : option (world * trace * atom * list tag) :=
   match bf with
   | Full =>
     match access_mode ty with
     | By_value chunk =>
       match type_is_volatile ty with
-      | false => do v <- Mem.loadv chunk m (Vptr b ofs); Some(w, E0, v)
-      | true => do_volatile_load w chunk m b ofs
+      | false => do v <- Mem.loadv chunk m (Vptr b ofs); Some(w, E0, v, loadv_ltags chunk m (Vptr b ofs))
+      | true => option_map (fun x => (x,[])) (do_volatile_load w chunk m b ofs)
       end
-    | By_reference => Some(w, E0, Vptr b ofs)
-    | By_copy => Some(w, E0, Vptr b ofs)
+    | By_reference => Some(w, E0, (Vptr b ofs,pt), [])
+    | By_copy => Some(w, E0, (Vptr b ofs,pt),[])
     | _ => None
     end
   | Bits sz sg pos width =>
@@ -293,7 +322,8 @@ Definition do_deref_loc (w: world) (ty: type) (m: mem) (b: block) (ofs: ptrofs) 
              signedness_eq sg1 (if zlt width (bitsize_intsize sz) then Signed else sg) &&
              zle 0 pos && zlt 0 width && zle width (bitsize_intsize sz) && zle (pos + width) (bitsize_carrier sz));
       match Mem.loadv (chunk_for_carrier sz) m (Vptr b ofs) with
-      | Some (Vint c) => Some (w, E0, Vint (bitfield_extract sz sg pos width c))
+      | Some (Vint c,vt) => Some (w, E0, (Vint (bitfield_extract sz sg pos width c),vt),
+                                   loadv_ltags (chunk_for_carrier sz) m (Vptr b ofs))
       | _ => None
       end
     | _ => None
@@ -301,49 +331,49 @@ Definition do_deref_loc (w: world) (ty: type) (m: mem) (b: block) (ofs: ptrofs) 
   end.
 
 Definition assign_copy_ok (ty: type) (b: block) (ofs: ptrofs) (b': block) (ofs': ptrofs) : Prop :=
-  (alignof_blockcopy ge ty | Ptrofs.unsigned ofs') /\ (alignof_blockcopy ge ty | Ptrofs.unsigned ofs) /\
+  (alignof_blockcopy (snd ge) ty | Ptrofs.unsigned ofs') /\ (alignof_blockcopy (snd ge) ty | Ptrofs.unsigned ofs) /\
   (b' <> b \/ Ptrofs.unsigned ofs' = Ptrofs.unsigned ofs
-           \/ Ptrofs.unsigned ofs' + sizeof ge ty <= Ptrofs.unsigned ofs
-           \/ Ptrofs.unsigned ofs + sizeof ge ty <= Ptrofs.unsigned ofs').
+           \/ Ptrofs.unsigned ofs' + sizeof (snd ge) ty <= Ptrofs.unsigned ofs
+           \/ Ptrofs.unsigned ofs + sizeof (snd ge) ty <= Ptrofs.unsigned ofs').
 
 Remark check_assign_copy:
   forall (ty: type) (b: block) (ofs: ptrofs) (b': block) (ofs': ptrofs),
   { assign_copy_ok ty b ofs b' ofs' } + {~ assign_copy_ok ty b ofs b' ofs' }.
 Proof with try (right; intuition lia).
   intros. unfold assign_copy_ok.
-  destruct (Zdivide_dec (alignof_blockcopy ge ty) (Ptrofs.unsigned ofs')); auto...
-  destruct (Zdivide_dec (alignof_blockcopy ge ty) (Ptrofs.unsigned ofs)); auto...
+  destruct (Zdivide_dec (alignof_blockcopy (snd ge) ty) (Ptrofs.unsigned ofs')); auto...
+  destruct (Zdivide_dec (alignof_blockcopy (snd ge) ty) (Ptrofs.unsigned ofs)); auto...
   assert (Y: {b' <> b \/
               Ptrofs.unsigned ofs' = Ptrofs.unsigned ofs \/
-              Ptrofs.unsigned ofs' + sizeof ge ty <= Ptrofs.unsigned ofs \/
-              Ptrofs.unsigned ofs + sizeof ge ty <= Ptrofs.unsigned ofs'} +
+              Ptrofs.unsigned ofs' + sizeof (snd ge) ty <= Ptrofs.unsigned ofs \/
+              Ptrofs.unsigned ofs + sizeof (snd ge) ty <= Ptrofs.unsigned ofs'} +
            {~(b' <> b \/
               Ptrofs.unsigned ofs' = Ptrofs.unsigned ofs \/
-              Ptrofs.unsigned ofs' + sizeof ge ty <= Ptrofs.unsigned ofs \/
-              Ptrofs.unsigned ofs + sizeof ge ty <= Ptrofs.unsigned ofs')}).
+              Ptrofs.unsigned ofs' + sizeof (snd ge) ty <= Ptrofs.unsigned ofs \/
+              Ptrofs.unsigned ofs + sizeof (snd ge) ty <= Ptrofs.unsigned ofs')}).
   destruct (eq_block b' b); auto.
   destruct (zeq (Ptrofs.unsigned ofs') (Ptrofs.unsigned ofs)); auto.
-  destruct (zle (Ptrofs.unsigned ofs' + sizeof ge ty) (Ptrofs.unsigned ofs)); auto.
-  destruct (zle (Ptrofs.unsigned ofs + sizeof ge ty) (Ptrofs.unsigned ofs')); auto.
+  destruct (zle (Ptrofs.unsigned ofs' + sizeof (snd ge) ty) (Ptrofs.unsigned ofs)); auto.
+  destruct (zle (Ptrofs.unsigned ofs + sizeof (snd ge) ty) (Ptrofs.unsigned ofs')); auto.
   right; intuition lia.
   destruct Y... left; intuition lia.
 Defined.
 
-Definition do_assign_loc (w: world) (ty: type) (m: mem) (b: block) (ofs: ptrofs) (bf: bitfield) (v: val): option (world * trace * mem * val) :=
+Definition do_assign_loc (w: world) (ty: type) (m: mem) (b: block) (ofs: ptrofs) (pt:tag) (bf: bitfield) (v: atom) (lts: list tag) : option (world * trace * mem * atom) :=
   match bf with
   | Full =>
     match access_mode ty with
     | By_value chunk =>
         match type_is_volatile ty with
-        | false => do m' <- Mem.storev chunk m (Vptr b ofs) v; Some(w, E0, m', v)
-        | true => do_volatile_store w chunk m b ofs v
+        | false => do m' <- Mem.storev chunk m (Vptr b ofs) v lts; Some(w, E0, m', v)
+        | true => do_volatile_store w chunk m b ofs v lts
         end
     | By_copy =>
         match v with
-        | Vptr b' ofs' =>
+        | (Vptr b' ofs',vt) =>
             if check_assign_copy ty b ofs b' ofs' then
-              do bytes <- Mem.loadbytes m b' (Ptrofs.unsigned ofs') (sizeof ge ty);
-              do m' <- Mem.storebytes m b (Ptrofs.unsigned ofs) bytes;
+              do bytes <- Mem.loadbytes m b' (Ptrofs.unsigned ofs') (sizeof (snd ge) ty);
+              do m' <- Mem.storebytes m b (Ptrofs.unsigned ofs) bytes lts;
               Some(w, E0, m', v)
             else None
         | _ => None
@@ -353,40 +383,45 @@ Definition do_assign_loc (w: world) (ty: type) (m: mem) (b: block) (ofs: ptrofs)
   | Bits sz sg pos width =>
     check (zle 0 pos && zlt 0 width && zle width (bitsize_intsize sz) && zle (pos + width) (bitsize_carrier sz));
     match ty, v, Mem.loadv (chunk_for_carrier sz) m (Vptr b ofs) with
-    | Tint sz1 sg1 _, Vint n, Some (Vint c) =>
+    | Tint sz1 sg1 _, (Vint n,vt), Some (Vint c,ovt) =>
         check (intsize_eq sz1 sz &&
                signedness_eq sg1 (if zlt width (bitsize_intsize sz) then Signed else sg));
         do m' <- Mem.storev (chunk_for_carrier sz) m (Vptr b ofs)
-                            (Vint ((Int.bitfield_insert (first_bit sz pos width) width c n)));
-        Some (w, E0, m', Vint (bitfield_normalize sz sg width n))
+                            (Vint ((Int.bitfield_insert (first_bit sz pos width) width c n)),vt) lts;
+        Some (w, E0, m', (Vint (bitfield_normalize sz sg width n),vt))
     | _, _, _ => None
     end
   end.
 
 Lemma do_deref_loc_sound:
-  forall w ty m b ofs bf w' t v,
-  do_deref_loc w ty m b ofs bf = Some(w', t, v) ->
-  deref_loc ge ty m b ofs bf t v /\ possible_trace w t w'.
+  forall w ty m b ofs pt bf w' t v vt lts,
+  do_deref_loc w ty m b ofs pt bf = Some(w', t, (v,vt), lts) ->
+  deref_loc ge ty m b ofs pt bf t (v,vt) lts /\ possible_trace w t w'.
 Proof.
-  unfold do_deref_loc; intros until v.
+  unfold do_deref_loc; intros until lts.
   destruct bf.
 - destruct (access_mode ty) eqn:?; mydestr.
-  intros. exploit do_volatile_load_sound; eauto. intuition. eapply deref_loc_volatile; eauto.
+  intros. exploit do_volatile_load_sound; eauto.
+  destruct (do_volatile_load w m0 m b ofs) eqn:?; simpl in H; inv H. eauto.
+  intuition. eapply deref_loc_volatile; eauto.
   split. eapply deref_loc_value; eauto. constructor.
   split. eapply deref_loc_reference; eauto. constructor.
   split. eapply deref_loc_copy; eauto. constructor.
 - mydestr. destruct ty; mydestr. InvBooleans. subst i. destruct v0; mydestr.
-  split. eapply deref_loc_bitfield; eauto. econstructor; eauto. constructor.
+  split.
+  + eapply deref_loc_bitfield; eauto. econstructor; eauto.
+  + constructor.
 Qed.
 
 Lemma do_deref_loc_complete:
-  forall w ty m b ofs bf w' t v,
-  deref_loc ge ty m b ofs bf t v -> possible_trace w t w' ->
-  do_deref_loc w ty m b ofs bf = Some(w', t, v).
+  forall w ty m b ofs pt bf w' t v vt lts,
+    deref_loc ge ty m b ofs pt bf t (v,vt) lts -> possible_trace w t w' ->
+    do_deref_loc w ty m b ofs pt bf = Some(w', t, (v,vt), lts).
 Proof.
   unfold do_deref_loc; intros. inv H.
-- inv H0. rewrite H1; rewrite H2; rewrite H3; auto.
-- rewrite H1; rewrite H2. apply do_volatile_load_complete; auto.
+  - inv H0. rewrite H3; rewrite H4. unfold loadv. rewrite H7; auto.
+  - rewrite H3; rewrite H6. apply (do_volatile_load_complete w _ _ _ _ w') in H8.
+    rewrite H8. simpl.
 - inv H0. rewrite H1. auto.
 - inv H0. rewrite H1. auto.
 - inv H0. inv H1.
